NumLean/Data/HTuple.lean
@@ -1,5 +1,6 @@
 import NumLean.Data.HTuple.Basic
 import NumLean.Data.HTuple.Ops
 import NumLean.Data.HTuple.Algebra
+import NumLean.Data.HTuple.HTupleMap
 import NumLean.Data.HTuple.RangeIterator
 import NumLean.Data.HTuple.RangeNotation
